heap/math_prop.v
@@ -1,0 +1,32 @@
+Require Import FloydSeq.proofauto.
+(* Require Import cprogs.heap.program. *)
+Require Import Notations Logic Datatypes.
+From Coq Require Import String List ZArith. 
+From compcert Require Import Coqlib Integers Floats AST Ctypes Cop Clight Clightdefs.
+Require Import Coq.Logic.Classical_Pred_Type.
+Require Import Coq.Logic.Classical_Prop.
+
+Require Import Coq.micromega.Psatz.
+Local Open Scope string.
+Local Open Scope nat_scope.
+Local Open Scope Z_scope.
+Local Open Scope list_scope.
+
+Require Import SetsClass.SetsClass.
+Local Open Scope sets.
+Import SetsNotation.
+
+Lemma Div_2_gt_0: forall (n: Z), 
+  1 <= n/2 -> n/2 < n.
+Proof.
+Admitted.
+
+Lemma Odd_Div2: forall (n: Z),
+  n >= 1 -> (n*2+1)/2 = n.
+Proof.
+Admitted.
+
+Lemma Even_Div2: forall (n: Z),
+  n >= 1 -> (n*2)/2 = n.
+Proof.
+Admitted.
