heap/tree_push.v
@@ -1,0 +1,728 @@
+Require Import FloydSeq.proofauto.
+(* Require Import cprogs.heap.program. *)
+Require Import Notations Logic Datatypes.
+From Coq Require Import String List ZArith. 
+From compcert Require Import Coqlib Integers Floats AST Ctypes Cop Clight Clightdefs.
+Require Import Coq.Logic.Classical_Pred_Type.
+Require Import Coq.Logic.Classical_Prop.
+
+Require Import Coq.micromega.Psatz.
+Local Open Scope string.
+Local Open Scope nat_scope.
+Local Open Scope Z_scope.
+Local Open Scope list_scope.
+Require Import cprogs.heap.list_relation.
+Require Import cprogs.heap.definitions.
+Require Import cprogs.heap.tree_list.
+Require Import cprogs.heap.math_prop.
+Require Import cprogs.heap.tree_up.
+
+Require Import SetsClass.SetsClass.
+Local Open Scope sets.
+Import SetsNotation.
+(* 
+Inductive list_nth_on_partial_tree (l: list Z) (n: Z) (p: Z) (lt: partial_tree) : Prop :=
+  | nth_partial_tree_nil: p = n -> lt = nil -> list_nth_on_partial_tree l n p lt
+  | nth_partial_tree_cons: forall flg v t lt0, 
+    lt = (flg, v, t) :: lt0 ->
+    1 <= (p / 2) < Zlength l -> 
+    p = (p / 2) * 2 + (if flg then 1 else 0) ->
+    Znth (p / 2) l = v -> 
+    list_nth_on_tree l (p + (if flg then -1 else 1)) t -> 
+    list_nth_on_partial_tree l n (p / 2) lt0 -> 
+    list_nth_on_partial_tree l n p lt. *)
+
+(* Lemma list_nth_on_partial_tree_app: forall l n p lt (flg: bool) v t,
+  (if flg then
+    list_nth_on_partial_tree l (n * 2 + 1) p lt /\ list_nth_on_tree l (n * 2) t /\ Znth n l = v
+  else
+    list_nth_on_partial_tree l (n * 2) p lt /\ list_nth_on_tree l (n * 2 + 1) t /\ Znth n l = v) ->
+  1 <= n < Zlength l ->
+  list_nth_on_partial_tree l n p (lt ++ [(flg, v, t)]).
+Proof.
+  intros.
+  destruct flg.
+  {
+    revert l p v n t H H0.
+    induction lt; intros; simpl; destruct H as [? [? ?] ].
+    + inversion H; [ | discriminate].
+      pose proof Z.div_lt_upper_bound p 2 (n + 1) ltac:(lia) ltac:(lia).
+      pose proof Z.div_le_lower_bound p 2 n ltac:(lia) ltac:(lia).
+      eapply nth_partial_tree_cons; eauto; simpl.
+      * inversion H; [lia | discriminate].
+      * lia. 
+      * replace (p / 2) with n by lia; tauto.
+      * replace (p + -1) with (n * 2) by lia; tauto.
+      * apply nth_partial_tree_nil; [lia | tauto].
+    + destruct a as [[flga va] ta].
+      inversion H; [discriminate | ].
+      injection H3; intros; subst lt0 ta va flga.
+      eapply nth_partial_tree_cons; eauto.
+  }
+  {
+    revert l p v n t H H0.
+    induction lt; intros; simpl; destruct H as [? [? ?] ].
+    + inversion H; [ | discriminate].
+      pose proof Z.div_lt_upper_bound p 2 (n + 1) ltac:(lia) ltac:(lia).
+      pose proof Z.div_le_lower_bound p 2 n ltac:(lia) ltac:(lia).
+      eapply nth_partial_tree_cons; eauto; simpl.
+      * inversion H; [lia | discriminate].
+      * lia. 
+      * replace (p / 2) with n by lia; tauto.
+      * replace (p + 1) with (n * 2 + 1) by lia; tauto.
+      * apply nth_partial_tree_nil; [lia | tauto].
+    + destruct a as [[flga va] ta].
+      inversion H; [discriminate | ].
+      injection H3; intros; subst lt0 ta va flga.
+      eapply nth_partial_tree_cons; eauto.
+  }
+Qed. *)
+
+Lemma tree_push_decompose_sound: forall d t v,
+  complete_tree_push d t ->
+  exists pt, t = tree_compose pt Leaf /\ complete_tree_pop d (tree_compose pt (Node v Leaf Leaf)).
+Proof.
+  intros.
+  induction H.
+  + exists nil.
+    simpl.
+    split; [tauto |].
+    apply complete_tree_pop_right_hole.
+    - apply full_tree_Leaf; lia.
+    - apply complete_tree_pop_Leaf; lia. 
+  + destruct IHcomplete_tree_push as [pt [? ?]].
+    exists (pt ++ [(true, v0, ls)]); split.
+    - rewrite tree_compose_append, H1.
+      reflexivity.
+    - rewrite tree_compose_append. 
+      apply complete_tree_pop_right_hole; tauto.
+  + destruct IHcomplete_tree_push as [pt [? ?]].
+    exists (pt ++ [(false, v0, rs)]); split.
+    - rewrite tree_compose_append, H1.
+      reflexivity.
+    - rewrite tree_compose_append. 
+      apply complete_tree_pop_left_hole; tauto. 
+Qed.
+
+Lemma full_tree_equiv1: forall d t,
+  full_tree d t <-> full_tree_b d t = true.
+Proof.
+  intros.
+  split; intros.
+  + induction H; subst; simpl.
+    - reflexivity.
+    - rewrite IHfull_tree1, IHfull_tree2; reflexivity.
+  + revert d H.
+    induction t; simpl; intros.
+    - apply Z.eqb_eq in H; subst.
+      constructor; reflexivity.
+    - apply andb_prop in H; destruct H.
+      specialize (IHt1 _ H).
+      specialize (IHt2 _ H0).
+      constructor; auto.
+Qed.
+
+Lemma complete_tree_push_not_fullb: forall d t,
+  complete_tree_push d t ->
+  full_tree_b d t = false.
+Proof.
+  intros.
+  induction H; subst; simpl.
+  + reflexivity.
+  + apply andb_false_intro2; assumption.
+  + apply andb_false_intro1; assumption.
+Qed.
+
+Lemma full_tree_b_dep_restrict: forall t d,
+  full_tree_b d t = true -> full_tree_b (d + 1) t = false.
+Proof.
+  intros t.
+  induction t; simpl; intros.
+  + rewrite Z.eqb_neq.
+    rewrite Z.eqb_eq in H.
+    lia.
+  + apply andb_prop in H; destruct H.
+    specialize (IHt1 _ H).
+    replace (d - 1 + 1) with (d + 1 - 1) in IHt1 by lia.
+    apply andb_false_intro1; assumption. 
+Qed.
+
+Fixpoint tree_next_pow2 (d: Z) (tr: tree): Z :=
+  match tr with
+  | Leaf => 1
+  | Node v ls rs => 
+    if full_tree_b (d - 1) ls then
+      2 * tree_next_pow2 (d - 1) rs
+    else
+      2 * tree_next_pow2 (d - 1) ls
+  end.
+
+Lemma full_tree_nonneg: forall d t,
+  full_tree d t -> 0 <= d.
+Proof.
+  intros.
+  induction H; lia.
+Qed.
+
+Lemma full_tree_same_size: forall d t1 t2,
+  full_tree d t1 -> full_tree d t2 -> tree_size t1 = tree_size t2.
+Proof.
+  intros.
+  revert t2 H0.
+  induction H; intros.
+  + inversion H0; [reflexivity | ]. 
+    pose proof full_tree_nonneg _ _ H1; lia.
+  + inversion H1; subst.
+    - pose proof full_tree_nonneg _ _ H; lia.
+    - simpl.
+      rewrite (IHfull_tree1 _ H2).
+      rewrite (IHfull_tree2 _ H3).
+      reflexivity.  
+Qed.
+
+Lemma full_tree_next_pow2: forall d t,
+  full_tree d t ->
+  tree_next_pow2 (d + 1) t = tree_size t + 1.
+Proof.
+  intros.
+  induction H; simpl. 
+  + lia.
+  + replace (dep + 1 - 1) with dep by lia.
+    remember H as H'; clear HeqH'.
+    rewrite full_tree_equiv1 in H.
+    apply full_tree_b_dep_restrict in H.
+    replace (dep - 1 + 1) with dep in H by lia.
+    rewrite H; simpl.
+    replace (dep - 1 + 1) with dep in IHfull_tree1 by lia.
+    rewrite IHfull_tree1.
+    rewrite (full_tree_same_size _ _ _ H' H0).
+    lia.
+Qed.
+
+Lemma full_tree_next_index: forall d t, 
+  full_tree d t -> next_index (d + 1) 0 t = 0.
+Proof.
+  intros.
+  induction H; subst; simpl; auto.
+  replace (dep + 1 - 1) with dep by lia.
+  rewrite full_tree_equiv1 in H.
+  pose proof full_tree_b_dep_restrict _ _ H.
+  replace (dep - 1 + 1) with dep in H1 by lia.
+  rewrite H1; simpl.
+  replace (dep - 1 + 1) with dep in IHfull_tree1 by lia.
+  tauto.
+Qed.
+
+Lemma complete_tree_push_dep_positve: forall d t,
+  complete_tree_push d t -> 1 <= d.
+Proof.
+  intros.
+  induction H; lia.
+Qed.
+
+Lemma next_index_lowbit: forall n d t,
+  complete_tree_push d t ->
+  next_index d n t = n * (tree_next_pow2 d t) + next_index d 0 t.
+Proof.
+  intros.
+  revert d n H.
+  induction t; simpl; intros.
+  + lia.
+  + inversion H; subst v t1 t2.
+    - rewrite full_tree_equiv1 in H2.
+      rewrite H2; simpl.   
+      specialize (IHt2 (d - 1)).
+      remember IHt2 as IHt2'; clear HeqIHt2'.
+      specialize (IHt2' 1 H4).
+      rewrite IHt2'.
+      specialize (IHt2 (n * 2 + 1) H4).
+      rewrite IHt2.
+      lia. 
+    - pose proof complete_tree_push_not_fullb _ _ H2.
+      rewrite H0; simpl.   
+      specialize (IHt1 (d - 1) (n * 2) H2).
+      rewrite IHt1.
+      lia. 
+Qed.
+
+Lemma complete_tree_push_same_next_pow2: forall d t1 t2,
+  complete_tree_push d t1 -> complete_tree_push d t2 ->
+  tree_next_pow2 d t1 = tree_next_pow2 d t2.
+Proof.
+  intros.
+  revert t2 H0.
+  induction H; subst; simpl; intros.
+  + inversion H0; subst; simpl.
+    - reflexivity.
+    - pose proof complete_tree_push_dep_positve _ _ H1; lia.
+    - pose proof complete_tree_push_dep_positve _ _ H; lia.
+  + rewrite full_tree_equiv1 in H.
+    rewrite H; simpl.
+    inversion H1; subst; simpl.
+    - pose proof complete_tree_push_dep_positve _ _ H0; lia.
+    - rewrite full_tree_equiv1 in H2.
+      rewrite H2; simpl.
+      specialize (IHcomplete_tree_push _ H3).
+      lia.
+    - pose proof complete_tree_push_not_fullb _ _ H2.
+      rewrite H4; simpl.
+      specialize (IHcomplete_tree_push _ H2).
+      lia.
+  + pose proof complete_tree_push_not_fullb _ _ H.
+    rewrite H2; simpl.
+    inversion H1; subst; simpl.
+    - pose proof complete_tree_push_dep_positve _ _ H; lia.
+    - rewrite full_tree_equiv1 in H3. 
+      rewrite H3; simpl.
+      specialize (IHcomplete_tree_push _ H4).
+      lia.
+    - pose proof complete_tree_push_not_fullb _ _ H3.
+      rewrite H5; simpl.
+      specialize (IHcomplete_tree_push _ H3).
+      lia. 
+Qed.
+
+Lemma tree_next_index_size: forall t d,
+  complete_tree_push d t ->
+  next_index d 1 t = tree_size t + 1.
+Proof.
+  intros.
+  revert d H.
+  induction t; simpl; intros; [lia |].
+  inversion H; subst v t1 t2.
+  + remember H2 as H2'; clear HeqH2'.
+    rewrite full_tree_equiv1 in H2'.
+    rewrite H2'; simpl.
+    specialize (IHt2 (d - 1) H4).
+    rewrite next_index_lowbit by auto.
+    rewrite next_index_lowbit in IHt2 by auto.
+    pose proof full_tree_complete_tree_push _ _ H2.
+    replace (d - 1 + 1) with d in H0 by lia.
+    specialize (IHt1 d H0).
+    rewrite next_index_lowbit in IHt1 by auto.
+    pose proof full_tree_next_pow2 _ _ H2.
+    replace (d - 1 + 1) with d in H1 by lia.
+    pose proof complete_tree_push_same_next_pow2 _ _ _ H0 H.
+    simpl in H3; rewrite H2' in H3.
+    lia.
+  + pose proof complete_tree_push_not_fullb _ _ H2.
+    rewrite H0; simpl.
+    specialize (IHt1 (d - 1) H2).
+    rewrite next_index_lowbit by auto.
+    rewrite next_index_lowbit in IHt1 by auto.
+    pose proof full_tree_complete_tree_push _ _ H4.
+    replace (d - 2 + 1) with (d - 1) in H1 by lia.
+    specialize (IHt2 (d - 1) H1).
+    rewrite next_index_lowbit in IHt2 by auto.
+    pose proof full_tree_next_pow2 _ _ H4.
+    replace (d - 1 + 1) with d in H3 by lia.
+    pose proof complete_tree_push_same_next_pow2 _ _ _ H1 H2.
+    pose proof full_tree_next_index _ _ H4.
+    replace (d - 2 + 1) with (d - 1) in H6 by lia.
+    lia.     
+Qed.
+
+(* Lemma list_on_tree_compose: forall l n d t,
+  list_nth_on_tree l n t ->
+  complete_tree_push d t ->
+  exists pt, t = tree_compose pt Leaf /\
+  list_nth_on_partial_tree l n (next_index d n t) pt.
+Proof.
+  intros.
+  revert n H.
+  induction H0; intros.
+  + exists nil.
+    split; auto.
+    constructor; auto.
+  + inversion H1; subst v0 ls0 rs0.
+    specialize (IHcomplete_tree_push _ H8).
+    destruct IHcomplete_tree_push as [pt [? ?] ].
+    exists (pt ++ [(true, v, ls)]).
+    split.
+    - rewrite tree_compose_append.
+      rewrite H2.
+      auto.
+    - apply list_nth_on_partial_tree_app; [ | lia].
+      split; [ | split].
+      * simpl.
+        assert (full_tree_b (dep - 2) rs = false) by admit.
+        rewrite H4; tauto.
+      * tauto.
+      * tauto.
+  + inversion H1; subst v0 ls0 rs0.
+    specialize (IHcomplete_tree_push _ H7).
+    destruct IHcomplete_tree_push as [pt [? ?] ].
+    exists (pt ++ [(false, v, rs)]).
+    split.
+    - rewrite tree_compose_append.
+      rewrite H2.
+      auto.
+    - apply list_nth_on_partial_tree_app; [ | lia].
+      split; [ | split].
+      * simpl.
+        assert (full_tree_b (dep - 2) rs = true) by admit.
+        rewrite H4; tauto.
+      * tauto.
+      * tauto. 
+Admitted.
+
+Lemma list_on_tree_state_app: forall (l: list Z) (t: tree) (v: Z),
+  Zlength l >= 1 -> list_on_tree l t -> 
+  exists pt, list_on_tree_state (l++[v], Zlength l) (pt, Node v Leaf Leaf).
+Proof.
+  intros.
+  unfold list_on_tree in H0.
+  destruct H0 as [? [? [d ?]]].
+  unfold list_on_tree_state; simpl.
+  unfold list_on_tree_state_fix.
+  pose proof tree_push_trompose_sound _ _ v H2.
+  destruct H3 as [pt [? ?] ].
+  exists pt.
+  split.
+  + apply list_nth_on_tree_Node.
+    - rewrite Zlength_app.
+      replace (Zlength [v]) with 1 by auto.
+      lia.
+    - rewrite app_Znth2 by lia.
+      replace (Zlength l - Zlength l) with 0 by lia.
+      auto.
+    - constructor.
+    - constructor.
+  +      
+Qed. *)
+
+Lemma complete_tree_push_d_same: forall (t: tree) (d1 d2: Z), 
+  complete_tree_push d1 t -> complete_tree_push d2 t -> d1 = d2.
+Proof.
+  intros.
+  revert d1 d2 H0 H.
+  induction t; intros.
+  + inversion H.
+    inversion H0.
+    lia.
+  + inversion H; subst.
+    - inversion H0; subst.
+      * specialize (IHt2 _ _ H5 H7).
+        lia.
+      * pose proof full_tree_complete_tree_push _ _ H7.
+        replace (d2-2+1) with (d2-1) in H1 by lia.
+        specialize (IHt2 _ _ H5 H1).
+        lia.
+    - inversion H0; subst.
+      * pose proof full_tree_complete_tree_push _ _ H5.
+        replace (d1-2+1) with (d1-1) in H1 by lia.
+        specialize (IHt2 _ _ H1 H7).
+        lia.
+      * specialize (IHt1 _ _ H3 H4).
+        lia.
+Qed.
+
+Lemma list_nth_on_tree_app:  forall (l: list Z) (v n: Z) (t: tree),
+  list_nth_on_tree l n t -> list_nth_on_tree (l++[v]) n t.
+Proof.
+  intros.
+  induction H.
+  + apply list_nth_on_tree_Leaf.
+  + eapply list_nth_on_tree_Node; try tauto.
+    - rewrite Zlength_app.
+      replace (Zlength [v]) with 1 by tauto.
+      lia.
+    - rewrite app_Znth1; [tauto|lia].
+Qed.
+
+Lemma list_on_partial_tree_app: forall (l: list Z) (lt: partial_tree) (v n: Z),
+  list_on_partial_tree l n lt -> list_on_partial_tree (l ++ [v]) n lt.
+Proof.
+  intros.
+  revert n H.
+  induction lt; intros.
+  + inversion H; [|discriminate].
+    apply nil_partial_tree; tauto.
+  + destruct a as [[flg val] tr].
+    inversion H; [discriminate|].
+    injection H0; intros; subst.
+    eapply cons_partial_tree; try reflexivity; try tauto.
+    - rewrite Zlength_app.
+      replace (Zlength [v]) with 1 by tauto.
+      lia.
+    - rewrite app_Znth1; [tauto|lia].
+    - apply list_nth_on_tree_app; tauto.
+    - apply IHlt; tauto.
+Qed.
+
+Lemma list_on_tree_state_app2: forall (l: list Z) (t: tree) (lt: partial_tree) (v n  d: Z), 
+  list_on_tree_state (l,n) (lt,t) -> complete_tree_push d t ->
+  list_on_partial_tree (l++[v]) (next_index d n t) (tree_to_partial_tree_fix lt t d).
+Proof.
+  intros.
+  revert lt n d H H0.
+  induction t; intros.
+  + simpl.
+    unfold list_on_tree_state in H.
+    unfold list_on_tree_state_fix in H; simpl in H.
+    destruct H, H1, H2.
+    apply list_on_partial_tree_app; tauto.
+  + simpl.
+    remember (full_tree_b (d - 1) t1) as HQ.
+    destruct HQ; simpl.
+    - apply IHt2.
+      2: {
+        inversion H0; [tauto|].
+        pose proof full_tree_complete_tree_push _ _ H5.
+        replace (d-2+1) with (d-1) in H6 by lia.
+        tauto.
+      }
+      revert H; unfold list_on_tree_state.
+      unfold list_on_tree_state_fix; simpl; intros.
+      destruct H, H1, H2.
+      inversion H.
+      split; [tauto|].
+      split; [|tauto].
+      eapply cons_partial_tree; try reflexivity; try rewrite Odd_Div2; try lia.
+      * simpl.
+        replace (n * 2 + 1 + -1) with (n*2) by lia.
+        tauto.
+      * tauto.
+    - apply IHt1.
+      2: {
+        inversion H0; [|tauto].
+        apply full_tree_equiv1 in H3.
+        rewrite H3 in HeqHQ.
+        discriminate.
+      }
+      revert H; unfold list_on_tree_state.
+      unfold list_on_tree_state_fix; simpl; intros.
+      destruct H, H1, H2.
+      inversion H.
+      split; [tauto|].
+      split; [|tauto].
+      eapply cons_partial_tree; try reflexivity; try rewrite Even_Div2; try lia.
+      * simpl; tauto.
+      * tauto.
+Qed.
+
+Lemma tree_to_partial_tree_get: forall (t tr: tree) (lt: partial_tree) (flg: bool) (v d: Z), 
+  tree_to_partial_tree_fix (lt ++ [(flg,v,tr)]) t d = (tree_to_partial_tree_fix lt t d) ++ [(flg,v,tr)].
+Proof.
+  intros.
+  revert v tr flg d lt.
+  induction t; intros.
+  + unfold tree_to_partial_tree.
+    simpl. tauto.
+  + simpl.
+    destruct (full_tree_b (d - 1)).
+    - replace ((true, v, t1) :: (lt ++ [(flg, v0, tr)])) with ([(true, v, t1)] ++ (lt ++ [(flg, v0, tr)])) by reflexivity.
+      replace ((true, v, t1) :: lt) with ([(true, v, t1)] ++ lt) by reflexivity.
+      rewrite app_assoc.
+      apply IHt2.
+    - replace ((false, v, t2) :: (lt ++ [(flg, v0, tr)])) with ([(false, v, t2)] ++ (lt ++ [(flg, v0, tr)])) by reflexivity.
+      replace ((false, v, t2) :: lt) with ([(false, v, t2)] ++ lt) by reflexivity.
+      rewrite app_assoc.
+      apply IHt1.
+Qed.
+ 
+Lemma complete_tree_holds: forall (t: tree)(d v: Z), 
+  complete_tree_push d t -> complete_tree_pop d (tree_compose (tree_to_partial_tree t d) (Node v Leaf Leaf)). 
+Proof.
+  intros.
+  induction H; intros.
+  + subst; simpl.
+    apply complete_tree_pop_right_hole.
+    - apply full_tree_Leaf; lia.
+    - apply complete_tree_pop_Leaf; lia.  
+  + unfold tree_to_partial_tree.
+    apply full_tree_equiv1 in H.
+    simpl.
+    rewrite H.
+    replace ((true, v0, ls) :: nil) with (nil ++ [(true,v0,ls)]). 2: {
+      rewrite app_nil_l; auto.
+    }
+    rewrite tree_to_partial_tree_get.
+    rewrite tree_compose_append.
+    apply full_tree_equiv1 in H.
+    apply complete_tree_pop_right_hole; tauto.
+  + unfold tree_to_partial_tree.
+    pose proof complete_tree_push_not_fullb _ _ H.
+    simpl.
+    rewrite H1.
+    replace ((false, v0, rs) :: nil) with (nil ++ [(false,v0, rs)]). 2: {
+      rewrite app_nil_l; auto.
+    }
+    rewrite tree_to_partial_tree_get.
+    rewrite tree_compose_append.
+    apply full_tree_equiv1 in H0.
+    apply complete_tree_pop_left_hole; auto.
+    apply full_tree_equiv1 in H0.
+    auto.
+Qed.
+
+Lemma tree_to_partial_tree_size: forall (t: tree) (d: Z),
+  complete_tree_push d t -> tree_size t = partial_tree_size (tree_to_partial_tree t d).
+Proof.
+  intros.
+  revert d H.
+  induction t; intros.
+  + simpl; lia.
+  + unfold tree_to_partial_tree.
+    simpl.
+    inversion H; subst.
+    - rewrite full_tree_equiv1 in H2.
+      rewrite H2; simpl.
+      replace ((true, v, t1) :: nil) with (nil ++ [(true, v, t1)]); [|rewrite app_nil_l; auto]. 
+      rewrite tree_to_partial_tree_get.
+      rewrite partial_tree_append_size.
+      rewrite (IHt2 (d-1)); [reflexivity|tauto].
+    - pose proof complete_tree_push_not_fullb _ _ H2.
+      rewrite H0; simpl.
+      replace ((false, v, t2) :: nil) with (nil ++ [(false, v, t2)]); [|rewrite app_nil_l; auto]. 
+      rewrite tree_to_partial_tree_get.
+      rewrite partial_tree_append_size.
+      rewrite (IHt1 (d - 1)); [unfold tree_to_partial_tree; lia| auto]. 
+Qed.
+
+Lemma list_on_tree_state_app: forall (l: list Z) (t: tree) (v: Z),
+  Zlength l >= 1 -> list_on_tree l t -> exists d, list_on_tree_state (l++[v], Zlength l) (tree_to_partial_tree t d,Node v Leaf Leaf) /\ complete_tree_push d t.
+Proof.
+  intros.
+  unfold list_on_tree_state; simpl.
+  unfold list_on_tree_state_fix.
+  unfold list_on_tree in H0.
+  destruct H0, H1.
+  destruct H2 as [dep].
+  exists dep.
+  assert (Zlength (l ++ [v]) = Zlength l + 1). {
+    rewrite Zlength_app.
+    replace (Zlength [v]) with 1; [lia|].
+    unfold Zlength; unfold Zlength_aux; reflexivity.
+  }
+  split; [| tauto].
+  split.
+  + eapply list_nth_on_tree_Node.
+    - rewrite H3.
+      pose proof initial_world.zlength_nonneg _ l.
+      lia.
+    - rewrite app_Znth2; [|lia].
+      replace (Zlength l - Zlength l) with 0 by lia.
+      reflexivity.
+    - eapply list_nth_on_tree_Leaf. 
+    - eapply list_nth_on_tree_Leaf. 
+  + split.
+    assert (list_on_tree_state (l, 1) (nil, t)). {
+      unfold list_on_tree_state; simpl.
+      unfold list_on_tree_state_fix.
+      split; [tauto|].
+      split; [apply nil_partial_tree; reflexivity|].
+      split; simpl; [|exists dep]; tauto.
+    }
+    pose proof list_on_tree_state_app2 l t nil v 1 dep H4 H2.
+    - replace (Zlength l) with (tree_size t + 1) by lia.
+      unfold tree_to_partial_tree.
+      rewrite <- (tree_next_index_size _ dep); tauto.
+    - split.
+      * rewrite tree_compose_size.
+        rewrite <- (tree_to_partial_tree_size _ dep); [| tauto].
+        simpl.
+        rewrite Zlength_app.
+        replace (Zlength [v]) with 1 by tauto.
+        lia.
+      * apply complete_tree_equality.
+        pose proof complete_tree_holds _ _ v H2.
+        exists dep; tauto.
+Qed.
+
+Definition tree_push: tree -> Z -> tree -> Prop :=
+  fun t val t' =>
+    exists ts d d2, heap_tree_up ((tree_to_partial_tree t d), Node val Leaf Leaf) ts /\ complete_tree_push d t /\ t' = (tree_compose (fst ts) (snd ts)) /\ complete_tree_push d2 t'.
+
+Lemma tree_to_partial_tree_fix_hold: forall (lt: partial_tree) (t: tree) (d: Z),
+  MaxHeap_partial_tree lt -> MaxHeap t -> (t = Leaf \/ MaxHeap_partial_tree_v lt (get_tree_val t)) -> complete_tree_push d t -> MaxHeap_partial_tree (tree_to_partial_tree_fix lt t d).
+Proof.
+  intros.
+  revert lt d H H1 H2.
+  induction H0; intros.
+  + rewrite H.
+    simpl.
+    apply H0.
+  + subst.
+    destruct H3; [discriminate|].
+    simpl in H.
+    simpl.
+    inversion H4.
+    - apply full_tree_equiv1 in H6.
+      rewrite H6.
+      apply IHMaxHeap2; [ | |tauto].
+      * unfold MaxHeap_partial_tree; try tauto.
+      * destruct H1; [left; tauto|right].
+        eapply MaxHeap_partial_tree_v_app; try reflexivity; tauto.
+    - pose proof complete_tree_push_not_fullb _ _ H6.
+      rewrite H9.
+      apply IHMaxHeap1; [ | |tauto].
+      * unfold MaxHeap_partial_tree; try tauto.
+      * destruct H0; [left; tauto|right].
+        eapply MaxHeap_partial_tree_v_app; try reflexivity; tauto.
+Qed.
+
+Lemma MaxHeap_impl_MaxHeap_tree_up: forall (t: tree) (v d: Z),
+  MaxHeap t -> complete_tree_push d t -> MaxHeap_tree_up (tree_to_partial_tree t d,Node v Leaf Leaf).
+Proof.
+  intros.
+  revert d H H0.
+  induction t; intros.
+  + unfold tree_to_partial_tree.
+    unfold MaxHeap_tree_up.
+    simpl.
+    split; [tauto|].
+    split.
+    - eapply MaxHeap_Node; [reflexivity| | | | ]; tauto.
+    - exists v, Leaf, Leaf.
+      tauto.
+  + unfold MaxHeap_tree_up.
+    unfold fst, snd.
+    inversion H; [discriminate|].
+    injection H1; intros; subst.
+    split.
+      2: {
+        split; [|exists v, Leaf, Leaf; tauto].
+        eapply MaxHeap_Node; [reflexivity| | | |]; try tauto.
+        apply MaxHeap_Leaf; reflexivity.
+        apply MaxHeap_Leaf; reflexivity.
+      }
+      unfold tree_to_partial_tree.
+      apply tree_to_partial_tree_fix_hold; [unfold MaxHeap_partial_tree; tauto|tauto|right|tauto].
+      apply MaxHeap_partial_tree_v_nil; reflexivity.
+Qed.
+
+Lemma Push_tree_list_rel: forall (l l': list Z) (t: tree) (v: Z),
+  list_on_tree l t -> heap_push l v l' -> MaxHeap t ->
+  exists t', list_on_tree l' t' /\ MaxHeap t' /\ tree_push t v t'.
+Proof.
+  intros.
+  assert (Zlength l >= 1). {
+    unfold list_on_tree in H.
+    destruct H, H2.
+    pose proof tree_size_nonneg t.
+    lia.
+  }
+  unfold heap_push in H0.
+  destruct H0.
+  pose proof list_on_tree_state_app _ _ v H2 H.
+  destruct H3 as [d].
+  destruct H3.
+  pose proof MaxHeap_impl_MaxHeap_tree_up _ v d H1 H4.
+  pose proof Up_tree_list_rel _ _ _ H3 H0 H5.
+  destruct H6 as [t'].
+  destruct H6, H7.
+  pose proof list_on_tree_state_impl_tree_compose _ _ H7.
+  simpl in H9.
+  exists (tree_compose (fst t') (snd t')).
+  split; [tauto|].
+  split; [tauto|].
+  unfold tree_push.
+  unfold list_on_tree in H9.
+  destruct H9, H10.
+  destruct H11 as [d2].
+  exists t', d, d2.
+  split; [tauto|].
+  split; [tauto|].
+  split; [reflexivity|tauto].
+Qed.
